Tap

FreydSSA/Subst.lean
@@ -20,7 +20,31 @@ def InstSet.Subst.fromTuple {Φ : InstSet (Ty α)} {Γ Δ : Ctx ν (Ty α)}
   (f: (i : Fin Δ.length) → Φ.Tm 1 Γ (Δ.get i).ty) : Φ.Subst Γ Δ
   := match Δ with
   | [] => nil _
-  | x::Δ => cons (f ⟨0, by simp⟩) (fromTuple (λi => f i.succ))
+  | v::Δ => cons (f ⟨0, by simp⟩) (fromTuple (λi => f i.succ))
+
+def InstSet.Subst.get {Φ : InstSet (Ty α)} {Γ Δ : Ctx ν (Ty α)}
+  : Φ.Subst Γ Δ → (i : Fin Δ.length) → Φ.Tm 1 Γ (Δ.get i).ty
+  | cons e _, ⟨0, _⟩ => e
+  | cons _ σ, ⟨n + 1, hn⟩ => σ.get ⟨n, Nat.lt_of_succ_lt_succ hn⟩
+
+theorem InstSet.Subst.fromTuple_get {Φ : InstSet (Ty α)} {Γ Δ : Ctx ν (Ty α)}
+  : (σ : Φ.Subst Γ Δ) → fromTuple (σ.get) = σ
+  | nil _ => rfl
+  | cons e σ => by simp only [fromTuple, get, Fin.succ, fromTuple_get σ]
+
+theorem InstSet.Subst.get_fromTuple {Φ : InstSet (Ty α)} {Γ Δ : Ctx ν (Ty α)}
+  (σ : (i : Fin Δ.length) → Φ.Tm 1 Γ (Δ.get i).ty) : get (fromTuple σ) = σ
+  := by induction Δ with
+  | nil => funext i; nomatch i
+  | cons v Δ I =>
+    funext ⟨i, hi⟩
+    cases i <;> simp only [fromTuple, get, Fin.succ, *]
+
+theorem InstSet.Subst.ext {Φ : InstSet (Ty α)} {Γ Δ : Ctx ν (Ty α)}
+  (σ τ : Φ.Subst Γ Δ)
+  (h : (i : Fin Δ.length) → σ.get i = τ.get i)
+  : σ = τ
+  := by rw [<-fromTuple_get σ, <-fromTuple_get τ]; congr; apply funext; apply h
 
 def InstSet.Subst.wk_entry {Φ : InstSet (Ty α)}
   {Γ Δ Ξ : Ctx ν (Ty α)} (w: Γ.Wk Δ) : Φ.Subst Δ Ξ → Φ.Subst Γ Ξ
@@ -39,7 +63,7 @@ def InstSet.Subst.var {Φ : InstSet (Ty α)}
   | cons e _ => e
 
 def InstSet.Tm.subst {Φ : InstSet (Ty α)} {p : Purity}
-  {Γ Δ : Ctx ν (Ty α)} (σ : Φ.Subst Γ Δ) {A : Ty α}
+  {Γ Δ : Ctx ν (Ty α)} {A : Ty α} (σ : Φ.Subst Γ Δ)
   : Φ.Tm p Δ A → Φ.Tm p Γ A
   | var _ w => σ.var w
   | op f e => op f (e.subst σ)
@@ -52,11 +76,93 @@ def InstSet.Subst.comp {Φ : InstSet (Ty α)}
   | nil _ => nil _
   | cons e τ => cons (e.subst σ) (σ.comp τ)
 
---TODO: Subst.comp_assoc
+theorem InstSet.Subst.comp_nil {Φ : InstSet (Ty α)}
+  {Γ Δ : Ctx ν (Ty α)} (σ: Φ.Subst Γ Δ)
+  : σ.comp (nil _) = nil _
+  := rfl
 
---TODO: Subst.id, Subst.comp_id _for Typed_
+theorem InstSet.Tm.subst_nil' {Φ: InstSet (Ty α)} {p : Purity} {A : Ty α}
+  {Γ : Ctx ν (Ty α)}
+  {σ : Φ.Subst Γ Γ}
+  (hΓ : Γ = [])
+  (t : Φ.Tm p Γ A) : t.subst σ = t := by induction t with
+  | var _ w => cases hΓ; cases w
+  | _ => simp [subst, *]
 
---TODO: Subst.ofWk, Subst.comp_wk, Subst.wk_comp, Subst.wk_comp_wk, etc.
+theorem InstSet.Tm.subst_nil {Φ: InstSet (Ty α)} {p : Purity} {A : Ty α}
+  {σ : Φ.Subst (@List.nil (Var ν _)) []}
+  (t : Φ.Tm p [] A) : t.subst σ = t
+  := subst_nil' rfl t
+
+theorem InstSet.Subst.nil_comp {Φ : InstSet (Ty α)}
+  {Γ : Ctx ν (Ty α)}
+  : (σ: Φ.Subst [] Γ) → (nil _).comp σ = σ
+  | nil _ => rfl
+  | cons e σ => by simp [comp, σ.nil_comp, Tm.subst_nil]
+
+def InstSet.Subst.id {Φ : InstSet (Ty α)}
+  {Γ : Ctx ν (Ty α)} (h : Γ.Nodup) : Φ.Subst Γ Γ
+  := fromTuple (λi => Tm.var 1 (h.get i))
+
+def InstSet.Subst.ofWk {Φ : InstSet (Ty α)}
+  {Γ Δ : Ctx ν (Ty α)} (w : Γ.Wk Δ) (hΔ : Δ.Nodup) : Φ.Subst Γ Δ
+  := fromTuple (λi => Tm.var 1 (w.comp (hΔ.get i)))
+
+def InstSet.Subst.cons2 {Φ : InstSet (Ty α)}
+  {Γ Δ : Ctx ν (Ty α)} {x : Var ν (Ty α)} (σ : Φ.Subst Γ Δ) (hx : Γ.Fresh x.name)
+  : Φ.Subst (x::Γ) (x::Δ)
+  := (σ.wk_entry (Ctx.Wk.skip hx (Ctx.Wk.refl Γ))).cons (Tm.var 1 (Ctx.Wk.head _ _))
+
+theorem InstSet.Subst.ofWk_refl {Φ : InstSet (Ty α)}
+  {Γ : Ctx ν (Ty α)} (hΓ : Γ.Nodup)
+  : @ofWk _ _ Φ _ _ (Ctx.Wk.refl Γ) hΓ = Subst.id hΓ
+  := by simp only [id, ofWk]; congr; funext i; congr; apply Ctx.Wk.allEq
+
+-- theorem InstSet.Subst.wk_comp_wk {Φ : InstSet (Ty α)}
+--   {Γ Δ Ξ : Ctx ν (Ty α)} (w : Γ.Wk Δ) (w' : Δ.Wk Ξ) (hΔ : Δ.Nodup)
+--   : (@ofWk _ _ Φ _ _ w hΔ).comp (ofWk w' (hΔ.wk w')) = (ofWk (w.comp w') sorry)
+--   := by induction w with
+--   | nil => cases w'; rfl
+--   | cons v w I => cases w' with
+--     | cons _ w' => simp [comp, ofWk, fromTuple, Tm.subst]
+--     | skip hx w' => sorry
+--   | skip hx w I => sorry
+
+-- theorem InstSet.Subst.comp_wk {Φ : InstSet (Ty α)}
+--   {Γ Δ Ξ : Ctx ν (Ty α)} (σ : Φ.Subst Γ Δ) (w : Δ.Wk Ξ) (hΞ : Ξ.Nodup)
+--   : σ.comp (ofWk w hΞ) = σ.wk_exit w
+--   := by induction w with
+--   | nil => cases σ; rfl
+--   | cons v w I => cases σ with
+--     | cons e σ =>
+--       rw [wk_exit, <-I _ hΞ.of_cons]
+--       apply ext
+--       intro ⟨i, hi⟩
+--       sorry
+--   | skip hx w I => sorry
+
+--TODO: Subst.comp_wk, Subst.wk_comp, Subst.wk_comp_wk, etc. for _Nodup_...
+
+--TODO: Subst.comp_id, Tm.subst_id
+
+-- def InstSet.Tm.subst_comp {Φ : InstSet (Ty α)} {p : Purity}
+--   {Γ Δ Ξ : Ctx ν (Ty α)} {A : Ty α} (σ : Φ.Subst Γ Δ) (τ : Φ.Subst Δ Ξ)
+--   (t : Φ.Tm p Ξ A)
+--   : (t.subst τ).subst σ = t.subst (σ.comp τ)
+--   := by induction t with
+--   | var p w => cases p with
+--     | pure => simp [subst]; sorry
+--     | impure => simp [subst]; sorry
+--   | _ => simp [subst, *]
+
+-- theorem InstSet.Subst.comp_assoc {Φ : InstSet (Ty α)}
+--   {Γ Δ Ξ Ω : Ctx ν (Ty α)} (σ: Φ.Subst Γ Δ) (τ: Φ.Subst Δ Ξ) (υ: Φ.Subst Ξ Ω)
+--   : (σ.comp τ).comp υ = σ.comp (τ.comp υ)
+--   := by induction υ with
+--   | nil _ => simp [comp]
+--   | cons e υ I =>
+--     simp [comp, I]
+--     sorry
 
 --TODO: Subst.Iso for alpha conversion...
 
